Computable primitives  (#859)

investigations/cava2/Expr.v
@@ -20,6 +20,9 @@ Require Import Coq.NArith.NArith.
 Require Import Coq.Strings.String.
 
 Require Import Cava.Types.
+Require Import Cava.Primitives.
+
+Local Open Scope N.
 
 Definition tvar : Type := type -> Type.
 Existing Class tvar.
@@ -39,8 +42,6 @@ Section Vars.
 
   | Delay: forall {x}, denote_type x -> Circuit x [x] x
 
-  | AddMod : nat -> Circuit [] [Nat; Nat] Nat
-
   | ElimBool: forall {s1 s2 x},
     Circuit [] [] Bit
     -> Circuit s1 [] x
@@ -55,6 +56,10 @@ Section Vars.
   | MakeTuple: forall {s1 s2 x y}, Circuit s1 [] x
     -> Circuit s2 [] y
     -> Circuit (s1++s2) [] (x**y)
+
+  | UnaryOp : forall {x r}, UnaryPrim x r -> var x -> Circuit [] [] r
+  | BinaryOp : forall {x y r}, BinaryPrim x y r -> var x -> var y -> Circuit [] [] r
+  | TernaryOp : forall {x y z r}, TernaryPrim x y z r -> var x -> var y -> var z -> Circuit [] [] r
   .
 End Vars.
 
@@ -116,47 +121,150 @@ Module ExprNotations.
   Notation "'if' i 'then' t 'else' e" := ((ElimBool i t e))
     (in custom expr at level 5, left associativity) : expr_scope.
 
-  (* Regression tests *)
-  Section Var.
-    Context {var : tvar}.
-
-    Definition fork2 {A} : Circuit [] [A] (A ** A) := {{
-      fun a => ( a, a)
-    }}.
-
-    Definition silly_id {A} : Circuit [] [A] A := {{
-      fun a => let '(x,y;z) := (a, `fork2` a) in z
-    }}.
-
-    Definition fst3 {A} : Circuit [] [A**A**A] A := {{
-      fun xyz => let '(x,y;z) := xyz in x
-    }}.
-
-    Definition ite_test {A} : Circuit [] [Bit; A] A := {{
-      fun flag a =>
-        if `silly_id` flag then (a) else a
-    }}.
-
-    Definition test {sz: nat}: Circuit (Nat**Nat) [] Nat := {{
-      let/delay '(x;y) := (y,x) initially ((0,1):denote_type (Pair Nat Nat)) in y
-    }}.
-
-    Definition test2 {sz: nat}: Circuit (Nat**Nat) [Nat**Nat] Nat := {{
-      fun xy =>
-      let '(x ; y) := xy in
-      let/delay '(z;w) :=
-        let t := x in
-        (w, z)
-        initially ((0,0):denote_type (Nat**Nat)) in
-        x
-    }}.
-
-    (* Function composition for single arg functions *)
-    Definition compose {s1 s2 x y z} (f: Circuit s1 [x] y) (g: Circuit s2 [y] z)
-      : Circuit (s1++s2) [x] z := {{
-      fun x => `g` ( `f` x )
-    }}.
-    (* Notation "f >=> g" := (compose f g) (at level 61, right associativity) : expr_scope. *)
-
-  End Var.
 End ExprNotations.
+
+Section Var.
+  Context {var : tvar}.
+
+  Definition val_of t : denote_type t -> denote_type t := id.
+  Definition val_N {sz}: N -> denote_type (BitVec sz) := id.
+
+  Definition False := Constant (false: denote_type Bit).
+  Definition _0 {sz} := Constant (val_of (BitVec sz) 0).
+  Definition _1 {sz} := Constant (val_of (BitVec sz) 1).
+  Definition _2 {sz} := Constant (val_of (BitVec sz) 2).
+
+  Class bitlike x :=
+  { eq : var x -> var x -> Circuit [] [] Bit
+  ; not : var x -> Circuit [] [] x
+  (* ; xor : var x -> var x -> Circuit [] [] x *)
+  (* ; and : var x -> var x -> Circuit [] [] x *)
+  (* ; add : var x -> var x -> Circuit [] [] x *)
+  }.
+
+  Import ExprNotations.
+  Instance bit_bitlike: bitlike Bit :=
+  { eq x y :=  {{ `BinaryOp BinEq x y` }}
+  ; not x := {{ `UnaryOp UnNot x` }}
+  }.
+  Instance bitvec_bitlike n: bitlike (BitVec n) :=
+  { eq x y :=  {{ `BinaryOp BinEq x y` }}
+  ; not x := {{ `UnaryOp UnBitVecNot x` }}
+  }.
+
+End Var.
+
+Existing Instance bit_bitlike.
+Existing Instance bitvec_bitlike.
+
+Section RegressionTests.
+  Import ExprNotations.
+
+  Context {var : tvar}.
+
+  Definition fork2 {A} : Circuit [] [A] (A ** A) := {{
+    fun a => ( a, a)
+  }}.
+
+  Definition silly_id {A} : Circuit [] [A] A := {{
+    fun a => let '(x,y;z) := (a, `fork2` a) in z
+  }}.
+
+  Definition fst3 {A} : Circuit [] [A**A**A] A := {{
+    fun xyz => let '(x,y;z) := xyz in x
+  }}.
+
+  Definition ite_test {A} : Circuit [] [Bit; A] A := {{
+    fun flag a =>
+      if `silly_id` flag then (a) else a
+  }}.
+
+  Definition inital_state {sz} := val_of (BitVec sz ** BitVec sz) (0,1)%N.
+
+  Definition test {sz: nat}: Circuit (BitVec 10**BitVec 10) [] (BitVec 10) := {{
+    let/delay '(x;y) := (y,x) initially inital_state in y
+  }}.
+
+  Definition test2 {sz: nat}: Circuit (BitVec sz ** BitVec sz) [BitVec sz ** BitVec sz ] (BitVec sz) := {{
+    fun xy =>
+    let '(x ; y) := xy in
+    let/delay '(z;w) :=
+      let t := x in
+      (w, z)
+      initially inital_state in
+      x
+  }}.
+
+  (* Function composition for single arg functions *)
+  Definition compose {s1 s2 x y z} (f: Circuit s1 [x] y) (g: Circuit s2 [y] z)
+    : Circuit (s1++s2) [x] z := {{
+    fun x => `g` ( `f` x )
+  }}.
+  (* Notation "f >=> g" := (compose f g) (at level 61, right associativity) : expr_scope. *)
+
+End RegressionTests.
+
+Module PrimitiveNotations.
+  Notation "x && y" := (
+    Let x (fun v1 => Let y (fun v2 => BinaryOp BinBitAnd v1 v2))
+  ) (in custom expr at level 20, left associativity) : expr_scope.
+  Notation "x || y" := (
+    Let x (fun v1 => Let y (fun v2 =>
+     BinaryOp BinBitOr v1 v2
+  ))) (in custom expr at level 20, left associativity) : expr_scope.
+  Notation "x >= y" := (
+    Let x (fun v1 => Let y (fun v2 =>
+    BinaryOp BinBitVecGte v1 v2
+  ))) (in custom expr at level 19, no associativity) : expr_scope.
+
+  Notation "! x" := (
+    Let x not
+  ) (in custom expr at level 20) : expr_scope.
+  Notation "x == y" := (
+    Let x (fun v1 => Let y (fun v2 =>
+      BinaryOp BinEq v1 v2
+  ))) (in custom expr at level 19, no associativity) : expr_scope.
+  Notation "x ^ y" := (
+    Let x (fun v1 => Let y (fun v2 =>
+      BinaryOp BinBitVecXor v1 v2
+  ))) (in custom expr at level 20, left associativity) : expr_scope.
+  Notation "x & y" := (
+    Let x (fun v1 => Let y (fun v2 =>
+      BinaryOp BinBitVecAnd v1 v2
+  ))) (in custom expr at level 20, left associativity) : expr_scope.
+  Notation "x + y" := (
+    Let x (fun v1 => Let y (fun v2 =>
+      BinaryOp BinBitVecAddU v1 v2
+  ))) (in custom expr at level 20, left associativity) : expr_scope.
+  Notation "x >>> y" := (
+    Let x (fun v1 => UnaryOp (UnVecRotateRight y) v1
+  )) (in custom expr at level 19, no associativity) : expr_scope.
+  Notation "x >> y" := (
+    Let x (fun v1 => UnaryOp (UnVecShiftRight y) v1
+  )) (in custom expr at level 19, no associativity) : expr_scope.
+  Notation "x <<+ y" := (
+    Let x (fun v1 => Let y (fun v2 =>
+      BinaryOp BinVecShiftInRight v1 v2
+    ))) (in custom expr at level 19, no associativity) : expr_scope.
+
+  Notation "x :> y" := (
+    Let x (fun v1 => Let y (fun v2 =>
+      BinaryOp BinVecCons v1 v2
+  ))) (in custom expr at level 19, right associativity) : expr_scope.
+
+  Notation "[ ]" := (Constant (simple_denote_to_denote (t:=Vec _ 0) nil)) (in custom expr at level 19) : expr_scope.
+
+  Import ExprNotations.
+  Definition index {var t n i}: Circuit (var:=var) [] [Vec t n; BitVec i] t :=
+    {{ fun vec index => `BinaryOp BinVecIndex vec index` }}.
+  Definition vec_as_tuple {var t n}: Circuit (var:=var) [] [Vec t (S n)] (ntuple t n) :=
+    {{ fun vec => `UnaryOp UnVecToTuple vec` }}.
+  Definition slice {var t n} (start length: nat): Circuit (var:=var) [] [Vec t n] (Vec t length) :=
+    {{ fun vec => `UnaryOp (UnVecSlice start length) vec` }}.
+  Definition replace {var t n i}: Circuit (var:=var) [] [Vec t n; BitVec i; t] (Vec t n) :=
+    {{ fun vec index val => `TernaryOp TernVecReplace vec index val` }}.
+
+End PrimitiveNotations.
+
+Axiom value_hole : forall {t}, t.
+Axiom circuit_hole : forall {t var}, Circuit (var:=var) [] [] t.
