investigations/cava2/Sha256.v
@@ -39,7 +39,7 @@ Section Var.
   Definition sha_digest := Vec sha_word 8.
 
   (* SHA-256 message padding *)
-  Definition sha256_padder : Circuit _ [Bit; Vec (BitVec 8) 4; Bit; Bit] (sha_word ** Bit) := {{
+  Definition sha256_padder : Circuit _ [Bit; BitVec 32; Bit; Bit] (sha_block ** Bit) := {{
     fun data_valid data finish clear =>
     (* TODO *)
     `circuit_hole`
@@ -88,16 +88,18 @@ Section Var.
   }}%nat.
 
   (* SHA-256 compression function *)
-  Definition sha256_compress : Circuit [] [sha_digest; sha_word; sha_word] sha_digest := {{
+  Program
+  Definition sha256_compress : Circuit []%circuit_type [sha_digest; sha_word; sha_word]%circuit_type sha_digest := {{
     fun current_digest k w =>
-    let '( a', b', c', d', e', f', g'; h' ) := `vec_as_tuple (n:=8)` current_digest in
+    let '( a', b', c', d', e', f', g'; h' ) := `vec_as_tuple (n:=7)` current_digest in
 
     let s1 := (e' >>> `6`) ^ (e' >>> `11`) ^ (e' >>> `25`) in
-    let ch := (e' & f') ^ (!e' & g') in
+    let ch := (e' & f') ^ (e' & g') in
     let temp1 := (h' + s1 + ch + k + w) in
     let s0 := (a' >>> `2`) ^ (a' >>> `13`) ^ (a' >>> `22`) in
     let maj := (a' & b') ^ (a' & c') ^ (b' & c') in
     let temp2 := s0 + maj in
+
 
     (temp1 + temp2) :> a' :> b' :> c' :> (d' + temp1) :> e' :> f' :> g' :> []
   }}%nat.
@@ -114,7 +116,7 @@ Section Var.
 
       let k_i := `sha256_round_constants` round in
       let '(w0,w1, _, _, _, _, _, _
-           , _,w9, _, _, _, _,w14;_ ) := `vec_as_tuple (n:=16)` message_schedule in
+           , _,w9, _, _, _, _,w14;_ ) := `vec_as_tuple (n:=15)` message_schedule in
       let update_schedule := round >= `Constant (16:denote_type (BitVec _))` in
       let w16 :=
         if update_schedule
@@ -143,3 +145,9 @@ Section Var.
 
 End Var.
 
+(* Section SanityCheck. *)
+(*   Require Import Cava.Semantics. *)
+(*   Time Compute step sha256_message_schedule_update tt (0,(3,(6,(9,tt)))). *)
+(*   Open Scope list_scope. *)
+(*   Time Compute step sha256_compress tt ([1;2;3;4;5;7;8;9],(1,(2,tt))). *)
+(* End SanityCheck. *)
